\subsubsection{Number Theory}


\begin{exercise}
    let $f(x) = a_nx^n + a_{n-1}x^{n-1} + .. + a_0$ be polynomial, and $a_k \in \mathbb{Z},\: a_n \ne 0,\: (a_0,a_1,..,a_n) = 1$

    and $g(x) = b_mx^m + b_{m-1}x^{m-1} + .. + b_0$ also be polynomial, and $b_k \in \mathbb{Z},\: b_m \ne 0,\: (b_0,b_1,..,b_m) = 1$

    prove: $f(x)g(x)$ is also a primitive polynomial.
\end{exercise}

\begin{proof}
    we expand $f(x)g(x)$ as:

    \[
        f(x)g(x) = c_0 + c_1x + .. + c_{n+m}x^{n+m}
    \]

    assume $f(x)g(x)$ is not primitive polynomial, there exists prime number $p$ and $p|c_k,\: \forall k \le n+m$

    let's consider $a_k$, since $f(x)$ is primitive we define:

    \[
        t_1 = \min \{ t: p  \nmid  a_t \}
    \]

    and


    \[
        t_2 = \min \{ t: p  \nmid  b_t \}
    \]

    consider $c_{t_1 + t_2}$:

    \begin{align*}
        c_{t_1+t_2} &\equiv \sum_{k+s = t_1+t_2}a_kb_s \equiv \sum_{\substack{k < t_1 \cup s < t_2 \\ k + s = t_1 + t_2}}a_kb_s + \sum_{\substack{k \ge t_1, s \ge t_2 \\ k+s = t_1+t_2}}a_kb_s \mod p \\ 
        & \equiv \sum_{\substack{k < t_1 \cup s < t_2 \\ k + s = t_1 + t_2}}0 + a_{t_1}b_{t_2} \mod p \\
    \end{align*}

    since $(p, a_{t_1}) = 1$ and $(p, b_{t_2}) = 1$ we got $(p,a_{t_1}b_{t_2}) = 1$ which is contradict with $p | c_{t_1 + t_2}$
\end{proof}